src/bbcache/BitBlastingCacheGeneral.v
@@ -1,0 +1,409 @@
+From Coq Require Import Arith ZArith OrderedType.
+From mathcomp Require Import ssreflect ssrfun ssrbool ssrnat eqtype seq.
+From nbits Require Import NBits.
+From ssrlib Require Import Types SsrOrder Var Nats ZAriths Tactics.
+From BitBlasting Require Import Typ TypEnv State QFBV CNF BBExport 
+     AdhereConform BitBlasting.
+From BBCache Require Import Cache BitBlastingCacheDef BitBlastingCacheNewer 
+     BitBlastingCachePreserve BitBlastingCacheCorrect BitBlastingCacheMkEnv 
+     BitBlastingCacheConsistent BitBlastingCacheSat BitBlastingCacheAdhere
+     BitBlastingCacheBound BitBlastingCache.
+
+Set Implicit Arguments.
+Unset Strict Implicit.
+Import Prenex Implicits.
+
+(* ================================================ *)
+(* ================================================ *)
+(* ======= bit-blasting with multiple bexps ======= *)
+(* ================================================ *)
+(* ================================================ *)
+
+
+(* ====== bit-blasting using a sequence of bexps ====== *)
+(* from the end of the sequence *)
+
+Fixpoint bit_blast_bexps_cache te (es : seq QFBV.bexp) :=
+  match es with 
+  | [::] => (init_vm, init_cache, init_gen, add_prelude [::], lit_tt)
+  | e :: es' => 
+    let '(m, ca, g, cs, lr) := bit_blast_bexps_cache te es' in
+    bit_blast_bexp_cache te m (reset_ct ca) g e
+  end.
+
+Fixpoint mk_env_bexps_cache (s : SSAStore.t) (es : seq QFBV.bexp) :=
+  match es with 
+  | [::] => (init_vm, init_cache, init_env, init_gen, add_prelude [::], lit_tt)
+  | e :: es' => 
+    let '(m, ca, E, g, cs, lr) := mk_env_bexps_cache s es' in
+    mk_env_bexp_cache m (reset_ct ca) s E g e
+  end.
+
+Fixpoint well_formed_bexps (bs : seq QFBV.bexp) te : bool :=
+  match bs with
+  | [::] => true
+  | b :: bs' => QFBV.well_formed_bexp b te && well_formed_bexps bs' te
+  end.
+
+Lemma mk_env_bexps_cache_newer_than_tt :
+  forall es s m ca E g cs lr, 
+    mk_env_bexps_cache s es = (m, ca, E, g, cs, lr) ->
+    newer_than_lit g lit_tt.
+Proof.
+  elim.
+  - move=> s m ca E g cs lr /=. case=> _ _ _ <- _ _. done.
+  - move=> e tl IHtl s m' ca' E' g' cs' lr'. 
+    rewrite /mk_env_bexps_cache -/mk_env_bexps_cache.
+    case Hmktl : (mk_env_bexps_cache s tl) => [[[[[m ca] E] g] cs] lr].
+    move=> Hmke.
+    move: (IHtl _ _ _ _ _ _ _ Hmktl) => Hgtt.
+    move: (mk_env_bexp_cache_newer_gen Hmke) => Hgg'.
+    exact: (newer_than_lit_le_newer Hgtt Hgg').
+Qed.
+
+Lemma mk_env_bexps_cache_newer_than_vm :
+  forall es s m ca E g cs lr, 
+    mk_env_bexps_cache s es = (m, ca, E, g, cs, lr) ->
+    newer_than_vm g m.
+Proof.
+  elim.
+  - move=> s m ca E g cs lr /=. case=> <- _ _ <- _ _. done.
+  - move=> e tl IHtl s m' ca' E' g' cs' lr'. 
+    rewrite /mk_env_bexps_cache -/mk_env_bexps_cache.
+    case Hmktl : (mk_env_bexps_cache s tl) => [[[[[m ca] E] g] cs] lr].
+    move=> Hmke.
+    move: (IHtl _ _ _ _ _ _ _ Hmktl) => Hgm.
+    exact: (mk_env_bexp_cache_newer_vm Hmke Hgm).
+Qed.
+
+Lemma mk_env_bexps_cache_tt :
+  forall es s m ca E g cs lr, 
+    mk_env_bexps_cache s es = (m, ca, E, g, cs, lr) ->
+    interp_lit E lit_tt.
+Proof.
+  elim.
+  - move=> s m ca E g cs lr /=. case=> _ _ <- _ _ _. done.
+  - move=> e tl IHtl s m' ca' E' g' cs' lr'. 
+    rewrite /mk_env_bexps_cache -/mk_env_bexps_cache.
+    case Hmktl : (mk_env_bexps_cache s tl) => [[[[[m ca] E] g] cs] lr].
+    move=> Hmke.
+    move: (mk_env_bexps_cache_newer_than_tt Hmktl) => Hgtt.
+    rewrite (env_preserve_lit (mk_env_bexp_cache_preserve Hmke) Hgtt).
+    exact: (IHtl _ _ _ _ _ _ _ Hmktl).
+Qed.
+
+
+(*
+Inductive bit_blast_bexps_cache_res te : 
+  vm -> cache -> generator -> cnf -> literal -> seq QFBV.bexp -> Prop :=
+(* | bbI : forall e m ca g cs lr,  *)
+(*     bit_blast_bexp_cache te init_vm init_cache init_gen e = (m, ca, g, cs, lr)  *)
+(*     -> QFBV.well_formed_bexp e te *)
+(*     -> bit_blast_bexps_cache_res te m ca g cs lr [::e] *)
+| bbI : bit_blast_bexps_cache_res te init_vm init_cache init_gen [::] lit_tt [::]
+| bbS : forall m ca g cs lr es e m' ca' g' cs' lr',
+    bit_blast_bexps_cache_res te m ca g cs lr es
+    -> bit_blast_bexp_cache te m (reset_ct ca) g e = (m', ca', g', cs', lr') 
+    -> QFBV.well_formed_bexp e te
+    -> bit_blast_bexps_cache_res te m' ca' g' cs' lr' (e::es).
+*)
+
+
+(* Lemma bit_blast_bexps_cache_res_well_formed : *)
+(*   forall es te m ca g cs lr, *)
+(*     bit_blast_bexps_cache_res te m ca g cs lr es -> *)
+(*     well_formed_bexps es te. *)
+(* Proof. *)
+(*   move=> es te m ca g cs lr Hbbes. *)
+(*   induction Hbbes as [| m ca g cs lr es e m' ca' g' cs' lr' Hbbes IH Hbbe Hwfe].  *)
+(*   - done. *)
+(*   - by rewrite /= Hwfe IH. *)
+(* Qed. *)
+
+Lemma mk_env_bexps_cache_is_bit_blast_bexps_cache :
+  forall es s te m ca E g cs lr,
+    mk_env_bexps_cache s es = (m, ca, E, g, cs, lr) ->
+    AdhereConform.conform_bexps es s te ->
+    well_formed_bexps es te ->
+    bit_blast_bexps_cache te es = (m, ca, g, cs, lr).
+Proof.
+  elim.
+  - move=> s te m ca E g cs lr /=. 
+    case=> <- <- _ <- <- <- _ _. done.
+  - move=> e es IHes s te m ca E g cs lr /=.
+    case Hmkes: (mk_env_bexps_cache s es) => [[[[[mes caes] Ees] ges] cses] lres].
+    move=> Hmke /andP [Hcfe Hcfes] /andP [Hwfe Hwfes].
+    move: (IHes _ te _ _ _ _ _ _ Hmkes Hcfes Hwfes) => Hbbes.
+    rewrite Hbbes.
+    exact: (mk_env_bexp_cache_is_bit_blast_bexp_cache Hcfe Hwfe Hmke).
+Qed.    
+
+Lemma mk_env_bexps_cache_consistent :
+  forall es s m ca E g cs lr,
+    mk_env_bexps_cache s es = (m, ca, E, g, cs, lr) ->
+    consistent m E s.
+Proof.
+  elim.
+  - move=> s m ca E g cs lr /=. case=> <- _ <- _ _ _. done.
+  - move=> e tl IHtl s m' ca' E' g' cs' lr'. 
+    rewrite /mk_env_bexps_cache -/mk_env_bexps_cache.
+    case Hmktl : (mk_env_bexps_cache s tl) => [[[[[m ca] E] g] cs] lr].
+    move=> Hmke.
+    move: (IHtl _ _ _ _ _ _ _ Hmktl) => HcmEs.
+    move: (mk_env_bexps_cache_newer_than_vm Hmktl) => Hgm.
+    exact: (mk_env_bexp_cache_consistent Hmke Hgm HcmEs). 
+Qed.
+
+
+
+Lemma mk_env_bexps_cache_well_formed :
+  forall es s m ca E g cs lr,
+    mk_env_bexps_cache s es = (m, ca, E, g, cs, lr) ->
+    Cache.well_formed ca.
+Proof.
+Admitted.
+
+Lemma mk_env_bexps_cache_newer_than_cache :
+  forall es s m ca E g cs lr,
+    mk_env_bexps_cache s es = (m, ca, E, g, cs, lr) ->
+    newer_than_cache g ca.
+Proof.
+Admitted.
+
+Lemma mk_env_bexps_cache_regular :
+  forall es s m ca E g cs lr,
+    mk_env_bexps_cache s es = (m, ca, E, g, cs, lr) ->
+    Cache.regular E ca.
+Proof.
+Admitted.
+
+Lemma mk_env_bexps_cache_sat :
+  forall es s m ca E g cs lr,
+    mk_env_bexps_cache s es = (m, ca, E, g, cs, lr) ->
+    interp_cnf E cs.
+Proof.
+  case.
+  - move=> s m ca E g cs lr /=. case=> _ _ <- _ <- _. done.
+  - move=> e tl s m' ca' E' g' cs' lr'. 
+    rewrite /mk_env_bexps_cache -/mk_env_bexps_cache.
+    case Hmktl : (mk_env_bexps_cache s tl) => [[[[[m ca] E] g] cs] lr].
+    move=> Hmke.
+    move: (mk_env_bexps_cache_newer_than_vm Hmktl) => Hgm.
+    move: (mk_env_bexps_cache_newer_than_tt Hmktl) => Hgtt.
+    (* move: (mk_env_bexps_cache_well_formed Hmktl) => Hwfca. *)
+    move: (reset_ct_well_formed ca) => Hwfrca.
+    move: (mk_env_bexps_cache_newer_than_cache Hmktl).
+    rewrite Cache.newer_than_cache_reset_ct => Hgrca.
+    move: (mk_env_bexps_cache_regular Hmktl).
+    rewrite Cache.regular_reset_ct => HrErca.
+    exact: (mk_env_bexp_cache_sat Hmke Hgm Hgtt Hwfrca Hgrca HrErca).
+Qed.
+
+Lemma mk_env_bexps_cache_correct :
+  forall es s m ca E g cs lr te,
+    mk_env_bexps_cache s es = (m, ca, E, g, cs, lr) ->
+    AdhereConform.conform_bexps es s te ->
+    well_formed_bexps es te ->
+    Cache.correct E s ca.
+Proof.
+  elim.
+  - move=> s m ca E g cs lr te /=. case=> _ <- <- _ _ _ _ _. done.
+  - move=> e tl IHtl s m' ca' E' g' cs' lr' te Hmk Hcf Hwf. 
+    move: (mk_env_bexps_cache_consistent Hmk) => HconmpEps.
+    move: (mk_env_bexps_cache_sat Hmk) => HiEpcsp.
+    move: (mk_env_bexps_cache_tt Hmk) => Htt.
+    have Hpre: interp_cnf E' (add_prelude cs')
+      by rewrite add_prelude_expand HiEpcsp Htt.
+    move: Hcf Hwf Hmk => /= /andP [Hcfe Hcftl] /andP [Hwfe Hwftl] {Htt HiEpcsp}.
+    case Hmktl : (mk_env_bexps_cache s tl) => [[[[[m ca] E] g] cs] lr].
+    move=> Hmke.
+    move: (mk_env_bexp_cache_is_bit_blast_bexp_cache Hcfe Hwfe Hmke) => Hbbe.
+    move: (IHtl _ _ _ _ _ _ _ _ Hmktl Hcftl Hwftl) => HcEsca.
+    move: (mk_env_bexp_cache_preserve Hmke) => HpEEpg.
+    move: (mk_env_bexps_cache_newer_than_cache Hmktl) => Hgca.
+    move: HcEsca. 
+    rewrite -(env_preserve_correct s HpEEpg Hgca) => {HpEEpg Hgca} HcEpsca.
+    move: (bit_blast_bexp_cache_correct_cache Hbbe Hcfe HconmpEps Hpre Hwfe 
+                                              (reset_ct_well_formed ca) HcEpsca).
+    by move=> [_ H].
+Qed.
+
+
+(* ===== generalized mk_env ===== *)
+
+Definition mk_envs_cache (s : SSAStore.t) (es : seq QFBV.bexp) : env :=
+  let '(m, ca, E, g, cs, lr) := mk_env_bexps_cache s es in
+  E.
+
+
+Lemma mk_envs_cache_tt :
+  forall es s, interp_lit (mk_envs_cache s es) lit_tt.
+Proof.
+  move=> es s. rewrite /mk_envs_cache.
+  case Hmkes : (mk_env_bexps_cache s es) => [[[[[m ca] E] g] cs] lr].  
+  exact: (mk_env_bexps_cache_tt Hmkes).
+Qed.
+
+
+Lemma mk_envs_cache_consistent :
+  forall es s te m ca g cs lr,
+    bit_blast_bexps_cache te es = (m, ca, g, cs, lr) ->
+    AdhereConform.conform_bexps es s te ->
+    well_formed_bexps es te ->
+    consistent m (mk_envs_cache s es) s.
+Proof.
+  move=> es s te m ca g cs lr Hbb Hcf Hwf.
+  rewrite /mk_envs_cache.
+  case Hmk: (mk_env_bexps_cache s es) => [[[[[m' ca'] E'] g'] cs'] lr'].
+  rewrite (mk_env_bexps_cache_is_bit_blast_bexps_cache Hmk Hcf Hwf) in Hbb.
+  case: Hbb => <- _ _ _ _.
+  exact: (mk_env_bexps_cache_consistent Hmk).
+Qed.
+
+
+Lemma mk_envs_cache_sat :
+  forall es s te m ca g cs lr,
+    bit_blast_bexps_cache te es = (m, ca, g, cs, lr) ->
+    AdhereConform.conform_bexps es s te ->
+    well_formed_bexps es te ->
+    interp_cnf (mk_envs_cache s es) cs.
+Proof.
+  move=> es s te m ca g cs lr Hbb Hcf Hwf.
+  rewrite /mk_envs_cache.
+  case Hmk: (mk_env_bexps_cache s es) => [[[[[m' ca'] E'] g'] cs'] lr'].
+  rewrite (mk_env_bexps_cache_is_bit_blast_bexps_cache Hmk Hcf Hwf) in Hbb.
+  case: Hbb => _ _ _ <- _.
+  exact: (mk_env_bexps_cache_sat Hmk).
+Qed.
+
+Lemma mk_envs_cache_correct :
+  forall es e s te m ca g cs lr,
+    bit_blast_bexps_cache te es = (m, ca, g, cs, lr) ->
+    AdhereConform.conform_bexps es s te ->
+    well_formed_bexps es te ->
+    Cache.correct (mk_envs_cache s (e::es)) s ca.
+Proof.
+  move=> es e s te m ca g cs lr Hbbes Hcf Hwf.
+  rewrite /mk_envs_cache /=.
+  case Hmkes: (mk_env_bexps_cache s es) => [[[[[m' ca'] E'] g'] cs'] lr'].
+  rewrite (mk_env_bexps_cache_is_bit_blast_bexps_cache Hmkes Hcf Hwf) in Hbbes.
+  case: Hbbes => _ <- _ _ _.
+  case Hmke: (mk_env_bexp_cache m' (reset_ct ca') s E' g' e)
+  => [[[[[me cae] Ee] ge] cse] lre].
+  move: (mk_env_bexps_cache_correct Hmkes Hcf Hwf) => HcEp.
+  move: (mk_env_bexps_cache_newer_than_cache Hmkes) => Hgpcap.
+  move: (mk_env_bexp_cache_preserve Hmke) => HpEpEe.
+  rewrite (env_preserve_correct s HpEpEe Hgpcap).
+  exact: HcEp.
+Qed.
+
+
+(*
+Lemma mk_envs_cache_correct :
+  forall es s te m ca g cs lr,
+    bit_blast_bexps_cache te es = (m, ca, g, cs, lr) ->
+    AdhereConform.conform_bexps es s te ->
+    well_formed_bexps es te ->
+    Cache.correct (mk_envs_cache s es) s ca.
+Proof.
+  elim.
+  - move=> s te m ca g cs lr /=. case=> _ <- _ _ _ _ _. done.
+  - move=> e tl IHtl s te m' ca' g' cs' lr' /=. 
+    (* move: (mk_envs_cache_consistent Hbb Hcf Hwf) => Hcon. *)
+    (* move: (mk_envs_cache_sat Hbb Hcf Hwf) => Hics'. *)
+    move=> Hbb /= /andP [Hcfe Hcftl] /andP [Hwfe Hwftl]. move: Hbb.
+    rewrite /mk_envs_cache -/mk_envs_cache /=.
+    case Hmktl : (mk_env_bexps_cache s tl) => [[[[[m ca] E] g] cs] lr].
+    move: (mk_env_bexps_cache_is_bit_blast_bexps_cache Hmktl Hcftl Hwftl) => Hbbtl.
+    rewrite Hbbtl. 
+    case Hmke : (mk_env_bexp_cache m (reset_ct ca) s E g e) 
+    => [[[[[me cae] Ee] ge] cse] lre].
+    move: (mk_env_bexp_cache_is_bit_blast_bexp_cache Hcfe Hwfe Hmke) => Hbbe.
+    rewrite Hbbe. case=> _ <- _ _ _.
+    move: (mk_env_bexps_cache_consistent Hmktl) => HcmEs.
+    move: (mk_env_bexps_cache_newer_than_vm Hmktl) => Hgm.
+    move: (mk_env_bexp_cache_consistent Hmke Hgm HcmEs) => HcmeEes.
+   Check bit_blast_bexp_cache_correct_cache.
+    
+move: (IHtl _ _ _ _ _ _ _ Hmktl) => HcEsca.
+    Check bit_blast_bexp_cache_correct_cache.
+    move:  bit_blast_bexp_cache_correct_cache.
+    move: (mk_env_bexps_cache_newer_than_vm Hmktl) => Hgm.
+    exact: (mk_env_bexp_cache_consistent Hmke Hgm HcmEs). 
+*)
+
+
+(* ===== Soundness and completeness ===== *)
+
+Theorem bit_blast_cache_general_sound :
+  forall (e : QFBV.bexp) (es : seq QFBV.bexp) te m ca g cs lr,
+    bit_blast_bexps_cache te (e::es) = (m, ca, g, cs, lr) ->
+    well_formed_bexps (e::es) te ->
+    ~ (sat (add_prelude ([::neg_lit lr]::cs))) ->
+    (forall s,
+        AdhereConform.conform_bexps (e::es) s te ->
+        QFBV.eval_bexp e s) .
+Proof.
+  move=> e es te m' ca' g' cs' lr' Hbb Hwf Hsat s Hcf.
+  move: (unsat_implies_valid Hsat) => {Hsat} Hsat.
+  move: (Hsat (mk_envs_cache s (e::es))) => {Hsat} Hsat.
+  move: (mk_envs_cache_sat Hbb Hcf Hwf) => Hcs. 
+  move: (mk_envs_cache_tt (e::es) s) => Htt.
+  have Hprelude: interp_cnf (mk_envs_cache s (e::es)) (add_prelude cs')
+    by rewrite add_prelude_expand Hcs Htt.
+  rewrite Hprelude /= in Hsat. 
+  move: (mk_envs_cache_consistent Hbb Hcf Hwf) => Hconmp.
+  move: Hbb => /=.
+  case Hbbes: (bit_blast_bexps_cache te es) => [[[[m ca] g] cs] lr].
+  move: Hwf Hcf => /= /andP [Hwfe Hwfes] /andP [Hcfe Hcfes] Hbbe. 
+  move: (mk_envs_cache_correct e Hbbes Hcfes Hwfes) => Hcr.
+  move: (bit_blast_bexp_cache_correct Hbbe Hcfe Hconmp Hprelude Hwfe
+                                      (reset_ct_well_formed ca) Hcr).
+  rewrite /enc_bit. move=> /eqP <-.
+  exact: Hsat.
+Qed.
+
+
+
+(* Definition correct_ct (E : env) (s : SSAStore.t) (c : cache) := *)
+(*   (forall e ls, ExpMap.find e (cet c) = Some ls -> enc_bits E ls (QFBV.eval_exp e s)) *)
+(*   /\ forall e l, BexpMap.find e (cbt c) = Some l -> enc_bit E l (QFBV.eval_bexp e s). *)
+
+
+(*
+Lemma bb_correct_test :
+  forall (e : QFBV.bexp) te m ca g m' ca' g' cs lr,
+    bit_blast_bexp_cache te m ca g e = (m', ca', g', cs, lr) ->
+    (* AdhereConform.conform_bexp e s te -> *)
+    QFBV.well_formed_bexp e te ->
+    Cache.well_formed ca -> strong_correct m ca ->    
+    enc_correct_bexp m' e cs lr.
+Proof.
+Admitted.
+
+Theorem bit_blast_cache_general_complete :
+  forall (e : QFBV.bexp) (es: seq QFBV.bexp) te m ca g cs lr,
+    bit_blast_bexps_cache te (e::es) = (m, ca, g, cs, lr) ->
+    well_formed_bexps (e::es) te ->
+    (forall s, AdhereConform.conform_bexps (e::es) s te ->
+               QFBV.eval_bexp e s)
+    ->
+    ~ (sat (add_prelude ([::neg_lit lr]::cs))).
+Proof.
+  move=> e es te m' ca' g' cs' lr' Hbb Hwf He.
+  move=> [E Hcs].
+  rewrite add_prelude_cons in Hcs. move/andP: Hcs => [Hlr Hcs].
+  rewrite add_prelude_expand in Hlr. move/andP: Hlr => [Htt Hlr].
+  rewrite /= interp_lit_neg_lit Bool.orb_false_r Bool.andb_true_r in Hlr. 
+  move : (bit_blast_bexp_cache_adhere (init_vm_adhere te) Hblast) => Hadm' .
+  move : (bit_blast_bexp_cache_bound Hblast init_well_formed_cache init_bound_cache)
+  => Hbound .
+  move : (mk_state_conform_bexp E Hbound Hadm') => Hcf .
+  move : (He (mk_state E m') Hcf) => {He} He .
+  move: (bit_blast_bexp_cache_correct Hblast Hcf (mk_state_consistent E m') 
+                                      Hcs Hwf init_well_formed_cache
+                                      (init_correct E (mk_state E m'))).
+  rewrite /enc_bit => /eqP H. rewrite -H in He.
+  rewrite He in Hlr. exact: not_false_is_true.
+Qed.
+*)
